# Solution 

## Q1) D 

## Q2) B

## Q3) C

## Q4) D 

## Q5) 

### A) {1, 2, 5, 6, 7}

### B) {3, 5}

### C) {2, 5, 7}

### D) {(1, 3), (1, 5), (3, 3), (3, 5), (6, 3), (6, 5)}

### E) 1


## Q6)

### assume f(x) is a bijective function then f(x) : R - {5} &rarr; R - {1} = f<sup>-1</sup>(x) : R - {1} &rarr; R - {5}

### We assume x = 2

### $$ { f(2) = 2 + 1 \over 2 - 5} = -1 $$

### Since f(x) = f<sup>-1</sup>(f(x))


### $$ { 2 \times f^{-1}(x)} = 4 $$  

### $$ { f^{-1}(x)}  = 2 $$  

### Since that $$ { f^{-1}(f(x)) } = x $$  

### Then we can see that f(x) has an inverse function so f(x) is bijective function